%
% d = c_11 c_22 - c_12 c_21
%
$ d^{_{12}D} = c_{12}c_{22} - c_{12}c_{22} = 0, $

$ d^{_{13}D} = c_{13}c_{22} - c_{12}c_{23} = d y_1, $

$ d^{_{23}D} = c_{11}c_{23} - c_{13}c_{21} = d y_2, $

$ d^{_{21}D} = c_{11}c_{21} - c_{11}c_{21} = 0, $

$ d^{_{31}D} = d^{_{32}D} = 0, $
\newline

%
% dy1 = c_22 c_13 - c_12 c_23
%
$ (d y_1)^{_{12}D} = (d y_1)^{_{13}D} = 0, $

$ (d y_1)^{_{23}D} = - c_{23}c_{13} + c_{13}c_{23} = 2 c_{13}c_{23}, $

$ (d y_1)^{_{21}D} = c_{21}c_{13} - c_{11}c_{23} = -d y_2, $

$ (d y_1)^{_{31}D} = c_{22}c_{11} - c_{12}c_{21} = d, $

$ (d y_1)^{_{32}D} = c_{22}c_{12} - c_{12}c_{22} = 0, $
\newline

%
% dy2 = c_11 c_23 - c_21 c_13
%
$ (d y_2)^{_{12}D} = c_{12}c_{23} - c_{22}c_{13} = -d y_1, $

$ (d y_2)^{_{13}D} = - c_{13}c_{23} + c_{23}c_{13} = - 2 c_{13}c_{23}, $

$ (d y_2)^{_{23}D} = (d y_2)^{_{21}D} = 0, $

$ (d y_2)^{_{31}D} = c_{11}c_{21} - c_{21}c_{11} = 0, $

$ (d y_2)^{_{32}D} = c_{11}c_{22} - c_{21}c_{12} = d. $