%
% Ri 12 D
%
$ r_i^{_{12}D} = (\lambda_1 - \lambda_2 - i) d^{\lambda_2 - 1} c_{11}^{\lambda_1 - \lambda_2 - i - 1} c_{12}^{i + 1} c_{33}^{\lambda_3} c_{13}c_{23} = (\lambda_1 - \lambda_2 - 1) r_{i + 1} $
\newline

%
% Ri 13 D
%
$ r_i^{_{13}D} = (\lambda_1 - \lambda_2 - i) d^{\lambda_2 - 1} c_{11}^{\lambda_1 - \lambda_2 - i - 1} c_{13} c_{12}^i c_{33}^{\lambda_3} c_{13}c_{23} + (\lambda_2 - 1) d^{\lambda_2 - 1} y_1 c_{11}^{\lambda_1 - \lambda_2 - i - 1} c_{13} c_{12}^i c_{33}^{\lambda_3} c_{13}c_{23} = ~0 $
\newline

%
% Ri 23 D
%
$ r_i^{_{23}D} = i d^{\lambda_2 - 1} c_{11}^{\lambda_1 - \lambda_2 - i} c_{13} c_{12}^{i - 1} c_{13} c_{33}^{\lambda_3} c_{13}c_{23} + (\lambda_2 - 1) d^{\lambda_2 - 1} y_2 c_{11}^{\lambda_1 - \lambda_2 - i - 1} c_{13} c_{12}^i c_{33}^{\lambda_3} c_{13}c_{23} = ~0 $
\newline

%
% Ri 21 D
%
$ r_i^{_{21}D} = i d^{\lambda_2 - 1} c_{11}^{\lambda_1 - \lambda_2 - i + 1} c_{12}^{i - 1} c_{33}^{\lambda_3} c_{13}c_{23} = i r_{i - 1} $
\newline

%
% Ri 31 D
%
$ r_i^{_{31}D} = d^{\lambda_2 - 1} c_{11}^{\lambda_1 - \lambda_2 - i} c_{12}^i (c_{33}^{\lambda_3} (c_{13}c_{21} - c_{11}c_{23}) + \lambda_3 c_{33}^{\lambda_3 - 1} c_{31}c_{13}c_{23}) = - u_i $
\newline

%
% Ri 32 D
%
$ r_i^{_{32}D} = d^{\lambda_2 - 1} c_{11}^{\lambda_1 - \lambda_2 - i} c_{12}^i (c_{33}^{\lambda_3} (c_{13}c_{22} - c_{12}c_{23}) + \lambda_3 c_{33}^{\lambda_3 - 1} c_{32}c_{13}c_{23}) = w_i $