$ v_i^{_{12}D} = (\lambda_1 - \lambda_2 - i)v_{i + 1}, $

$ v_i^{_{13}D} = (\lambda_1 + \lambda_3 - i)w_i + (\lambda_1 - \lambda_2 - i)u_{i + 1}, $

$ v_i^{_{23}D} = i w_{i - 1} + (\lambda_2 + \lambda_3 + i)u_i, $

$ v_i^{_{21}D} = i v_{i - 1}, v_i^{_{31}D} = v_i^{_{32}D} = 0 $
\newline

$ w_i^{_{12}D} = (\lambda_1 - \lambda_2 - i)w_{i + 1}, $

$ w_i^{_{13}D} = (\lambda_1 - \lambda_2 - i)r_{i + 1}, $

$ w_i^{_{23}D} = (\lambda_2 + \lambda_3 + i + 1)r_i, $

$ w_i^{_{21}D} = -u_i - i w_{i - 1}, w_i^{_{31}D} = v_i, w_i^{_{32}D} = 0, $
\newline

$ u_i^{_{12}D} = - w_i + (\lambda_1 - \lambda_2 - i)u_{i + 1}, $

$ u_i^{_{13}D} = (i - \lambda_1 - \lambda_3 - 1)r_i, $

$ u_i^{_{23}D} = -i r_{i - 1}, $

$ u_i^{_{21}D} = i u_{i - 1}, u_i^{_{31}D} = 0, u_i^{_{32}D} = v_i, $
\newline

$ r_i^{_{12}D} = (\lambda_1 - \lambda_2 - i)r_{i + 1}, $

$ r_i^{_{13}D} = r_i^{_{23}D} = 0, $

$ r_i^{_{21}D} = i r_{i - 1}, r_i^{_{31}D} = -u_i, r_i^{_{32}D} = w_i. $
